organizational update

messageInvariantPrototypes/ringLeaderElection/withoutMonotonic/hosts.dfy
@@ -1,4 +1,4 @@
-include "UtilitiesLibrary.dfy"
+include "../../lib/UtilitiesLibrary.dfy"
 
 module Types {
   import opened UtilitiesLibrary
@@ -24,7 +24,7 @@ module Host {
   }
 
   datatype Variables = Variables(
-    highestHeard: int
+    highestHeard: int   // monotonic int
   )
   {
     predicate WF(c: Constants) {
@@ -92,97 +92,3 @@ module Host {
     exists step :: NextStep(c, v, v', step, msgOps)
   }
 }  // end module Host
-
-module Network {
-  import opened Types
-
-  datatype Constants = Constants  // no constants for network
-
-  // Network state is the set of messages ever sent. Once sent, we'll
-  // allow it to be delivered over and over.
-  // (We don't have packet headers, so duplication, besides being realistic,
-  // also doubles as how multiple parties can hear the message.)
-  datatype Variables = Variables(sentMsgs:set<Message>)
-
-  predicate Init(c: Constants, v: Variables)
-  {
-    && v.sentMsgs == {}
-  }
-
-  predicate Next(c: Constants, v: Variables, v': Variables, msgOps: MessageOps)
-  {
-    // Only allow receipt of a message if we've seen it has been sent.
-    && (msgOps.recv.Some? ==> msgOps.recv.value in v.sentMsgs)
-    // Record the sent message, if there was one.
-    && v'.sentMsgs ==
-      v.sentMsgs + if msgOps.send.None? then {} else { msgOps.send.value }
-  }
-} // end module Network
-
-
-module DistributedSystem {
-  import opened Types
-  import Network
-  import Host
-
-  datatype Constants = Constants(
-    hostConstants: seq<Host.Constants>,
-    network: Network.Constants)
-  {
-    predicate ValidIdx(id: int) {
-      0 <= id < |hostConstants|
-    }
-
-    predicate UniqueIds() {
-      forall i, j | ValidIdx(i) && ValidIdx(j) && hostConstants[i].hostId == hostConstants[j].hostId :: i == j
-    }
-
-    predicate WF() {
-      && 0 < |hostConstants|
-      && UniqueIds()
-    }
-  }
-
-  datatype Variables = Variables(
-    hosts: seq<Host.Variables>,
-    network: Network.Variables)
-  {
-    predicate WF(c: Constants) {
-      && c.WF()
-      && Host.GroupWF(c.hostConstants, hosts)
-    }
-  }
-
-  predicate Init(c: Constants, v: Variables)
-  {
-    && v.WF(c)
-    && Host.GroupInit(c.hostConstants, v.hosts)
-    && Network.Init(c.network, v.network)
-  }
-
-  predicate HostAction(c: Constants, v: Variables, v': Variables, actorIdx: int, msgOps: MessageOps)
-  {
-    && v.WF(c)
-    && v'.WF(c)
-    && c.ValidIdx(actorIdx)
-    && Host.Next(c.hostConstants[actorIdx], v.hosts[actorIdx], v'.hosts[actorIdx], msgOps)
-    // all other hosts UNCHANGED
-    && (forall otherHostIdx | c.ValidIdx(otherHostIdx) && otherHostIdx != actorIdx :: v'.hosts[otherHostIdx] == v.hosts[otherHostIdx])
-  }
-
-  datatype Step = HostActionStep(actorIdx: int, msgOps: MessageOps)
-
-  predicate NextStep(c: Constants, v: Variables, v': Variables, step: Step)
-  {
-    && HostAction(c, v, v', step.actorIdx, step.msgOps)
-    // network agrees recv has been sent and records sent
-    && Network.Next(c.network, v.network, v'.network, step.msgOps)
-  }
-
-  predicate Next(c: Constants, v: Variables, v': Variables)
-  {
-    exists step :: NextStep(c, v, v', step)
-  }
-}  // end module DistributedSystem
-
-
