messageInvariantPrototypes/ringLeaderElection/withoutMonotonic/messageInvariants.dfy
@@ -2,7 +2,7 @@
 
 include "spec.dfy"
 
-module NetworkInvariants {
+module MessageInvariants {
   import opened Types
   import opened UtilitiesLibrary
   import opened DistributedSystem
@@ -22,14 +22,6 @@ module NetworkInvariants {
     :: msg.val >= c.hostConstants[msg.src].hostId
   }
 
-  // Every message's val less than or eq max(highest seen of nodes[msg.src], hostid of nodes[mag.src])
-  predicate payloadLeqSenderMax(c: Constants, v: Variables) 
-    requires v.WF(c)
-  {
-    forall msg | msg in v.network.sentMsgs && 0 <= msg.src < |c.hostConstants|
-    :: msg.val <= max(c.hostConstants[msg.src].hostId, v.hosts[msg.src].highestHeard)
-  }
-
   // For each host, if its highestHeard is >-1, then it must have gotten it from a message
   // from its predecessor
   predicate receiveValidity(c: Constants, v: Variables) 
@@ -42,24 +34,23 @@ module NetworkInvariants {
                       && idx == Successor(|c.hostConstants|, msg.src))
   }
 
-  predicate NetworkInv(c: Constants, v: Variables)
+  predicate MessageInv(c: Constants, v: Variables)
   {
     && v.WF(c)
     && VoteMsgValidSrc(c, v)
     && payloadGeqSenderHostId(c, v)
-    // && payloadLeqSenderMax(c, v)
     && receiveValidity(c, v)
   }
 
-  lemma InitImpliesNetworkInv(c: Constants, v: Variables)
+  lemma InitImpliesMessageInv(c: Constants, v: Variables)
     requires Init(c, v)
-    ensures NetworkInv(c, v)
+    ensures MessageInv(c, v)
   {}
 
-  lemma NetworkInvInductive(c: Constants, v: Variables, v': Variables)
-    requires NetworkInv(c, v)
+  lemma MessageInvInductive(c: Constants, v: Variables, v': Variables)
+    requires MessageInv(c, v)
     requires Next(c, v, v')
-    ensures NetworkInv(c, v')
+    ensures MessageInv(c, v')
   {}
 }
 
